theories/Core/Semantic/Readback/Lemmas.v
@@ -1,5 +1,6 @@
 From Coq Require Import Lia PeanoNat Relations.
-From Mcltt Require Import Base Evaluation LibTactics Readback.Definitions.
+From Mcltt Require Import Base LibTactics.
+From Mcltt.Core Require Import Evaluation Readback.Definitions.
 Import Domain_Notations.
 
 Section functional_read.
